Prove transfer gives transitivity and reflexivity

Bisimulations/Transfer.lean
@@ -1,11 +1,17 @@
+import Mathlib.Logic.Relation
 import Bisimulations.Relation
 
-variable {β : Sort l}
+variable {β : Type l}
 
 def Transfers {Obs : β → Sort k} (RT : RelT Obs) (R : Rel β) (p q : β) :=
   R p q → ∀ op : Obs p, ∃ oq : Obs q, RT R op oq
 
 variable {Obs : β → Sort k} {RT : RelT Obs} {R Q : Rel β}
+
+variable (RT) in
+class LawfulPosRelT extends LawfulRelT RT where
+  preserves_reflexivity : ∀ R, Reflexive R → DepReflexive (RT R)
+  preserves_transitivity : ∀ R, Transitive R → DepTransitive (RT R)
 
 lemma transfers_closed_under_union [laws : LawfulRelT RT]
     : Transfers RT R p q → Transfers RT Q p q → Transfers RT (RelCup R Q) p q := by
@@ -19,8 +25,42 @@ lemma transfers_closed_under_union [laws : LawfulRelT RT]
     apply laws.monotone _ _ right_subrel_rel_cup
     assumption
 
+lemma transfers_closed_under_reflexivity [laws : LawfulPosRelT RT]
+    : Transfers RT R p q → Transfers RT (Relation.ReflGen R) p q := by
+  rintro htransf (_ | hr) op
+  · exists op
+    apply laws.preserves_reflexivity
+    exact Relation.reflexive_reflGen
+  · rcases htransf hr op with ⟨oq, hr'⟩
+    exists oq
+    apply laws.monotone _ _ subrel_reflgen
+    assumption
+
 structure TransferRel (RT : RelT Obs) (R : Rel β) where
   transfer : ∀ ⦃p q : β⦄, Transfers RT R p q
+
+lemma transfer_rel_closed_under_transitivity [laws : LawfulPosRelT RT]
+    : TransferRel RT R → TransferRel RT (Relation.TransGen R) := by
+  intro ⟨htfs⟩
+  constructor
+  intro p _ hr
+  induction hr
+  case single q hr =>
+    intro op
+    rcases htfs hr op with ⟨oq, hr'⟩
+    exists oq
+    apply laws.monotone _ _ subrel_transgen
+    assumption
+  case tail q s hpq hqs ih =>
+    intro op
+    rcases ih op with ⟨oq, hpq'⟩
+    rcases htfs hqs oq with ⟨or, hqs'⟩
+    exists or
+    apply laws.preserves_transitivity
+    · exact Relation.transitive_transGen
+    · assumption
+    · apply laws.monotone _ _ subrel_transgen
+      assumption
 
 def transferRel (RT : RelT Obs) := Biggest (TransferRel RT)
 
