Bisimulations/SymmTransferDuality.lean
@@ -6,7 +6,7 @@ import Bisimulations.TransferDuality
 -- These theorems are very close to their original proofs; likely we can
 -- extend TransferRel with any property that is preserved by intersection,
 -- union, and complement, and prove all of them that way.
-variable {β : Sort l} {Obs : β → Sort k} {RT QT : RelT Obs} {R : Rel β}
+variable {β : Type l} {Obs : β → Sort k} {RT QT : RelT Obs} {R : Rel β}
 
 lemma symm_cotransfer_rel_of_compl_symm_transfer_rel [pair : DualRelTPair RT QT]
     : SymmTransferRel RT R → SymmCotransferRel QT (Compl R) := by
@@ -46,7 +46,6 @@ theorem symm_cotransfer_rel_iff_not_symm_transfer_rel [pair : DualRelTPair RT QT
   · apply not_symm_cotransfer_and_symm_transfer_rel
   · apply symm_cotransfer_rel_of_not_symm_transfer_rel
 
-open Classical in
 theorem symm_transfer_or_symm_cotransfer_rel [pair : DualRelTPair RT QT]
     : symmTransferRel RT p q ∨ symmCotransferRel QT p q := by
   cases em (symmTransferRel RT p q)
